different types of tracking oracles

src/computational_monads/asymptotics/queries_at_most.lean
@@ -4,30 +4,33 @@ import data.polynomial
 
 open oracle_comp oracle_spec
 
-variables {A : Type} {spec spec' : oracle_spec}
+variables {α β : Type} {spec spec' : oracle_spec}
 
 /-- Oracle computations that uniformly make at most a given number of queries.
   In particular `simulate` will call the `simulation_oracle` at most that many times -/
-inductive queries_at_most : Π {A : Type}, oracle_comp spec A → ℕ → Type 1
-| queries_at_most_sample {A : Type} (a : A) :
-    queries_at_most (pure' A a) 0
-| queries_at_most_bind' {A B : Type} (ca : oracle_comp spec A) (cb : A → oracle_comp spec B)
-    (p q : ℕ) (hca : queries_at_most ca p) (hcb : ∀ a, queries_at_most (cb a) q) :
-    queries_at_most (bind' A B ca cb) (p + q)
+inductive queries_at_most : Π {α : Type}, oracle_comp spec α → ℕ → Type 1
+| queries_at_most_sample {α : Type} (a : α) :
+    queries_at_most (pure a) 0
+| queries_at_most_bind' {α β : Type} (oa : oracle_comp spec α) (ob : α → oracle_comp spec β)
+    (p q : ℕ) (hca : queries_at_most oa p) (hcb : ∀ a, queries_at_most (ob a) q) :
+    queries_at_most (oa >>= ob) (p + q)
 | queries_at_most_query {i : spec.ι} (a : spec.domain i) :
-    queries_at_most (query i a) 1 
+    queries_at_most (query i a) 1
+| queries_at_most_trans {α : Type} (oa : oracle_comp spec α) {p q : ℕ}
+    (hoa : queries_at_most oa p) (h : p ≤ q) :
+    queries_at_most oa q
 
--- /-- Soundness of `queries_at_most` with respect to simulation -/
--- theorem queries_at_most_sound (oa : oracle_comp spec A)
---   (x : A × ℕ) (hx : x ∈ (default_simulate counting_oracle oa).support)
---   (n : ℕ) (hn : queries_at_most oa n) : x.2 ≤ n :=
--- begin
-
--- end
+/-- Soundness of `queries_at_most` with respect to simulation -/
+theorem queries_at_most_sound (oa : oracle_comp spec α) (x : α × ℕ)
+  (hx : x ∈ (default_simulate counting_oracle oa).support)
+  (n : ℕ) (hn : queries_at_most oa n) : x.2 ≤ n :=
+begin
+  sorry
+end
 
 /-- An function `ℕ → oracle_comp` has `polynomial_queries` if the number of queries made
   has growth bounded by a polynomial in the input `ℕ`. Note that it's a sigma type, not a `Prop`.
   Used to show that an `oracle_comp` with polynomial time simulated by a polynomial time oracle
     is still polynomial time if the number of queries is also polynomial -/
-def polynomial_queries (oa : ℕ → oracle_comp spec A) : Type 1 :=
+def polynomial_queries (oa : ℕ → oracle_comp spec α) : Type 1 :=
 Σ (p : polynomial ℕ), ∀ n, queries_at_most (oa n) (p.eval n)
