src/computational_monads/simulation_semantics/constructions/counting_oracle.lean
@@ -1,4 +1,4 @@
-import computational_monads.simulation_semantics.default_simulate
+import computational_monads.simulation_semantics.constructions.tracking_oracle
 
 /-!
 # Query Counting Simulation Oracle
@@ -12,9 +12,29 @@ This value is always finite as the `oracle_comp` monad doesn't have unbounded re
 open oracle_comp oracle_spec
 
 variables {α β γ : Type} {spec spec' : oracle_spec}
+  (oa : oracle_comp spec α) (ob : α → oracle_comp spec β) (n m : ℕ)
 
 /-- Simulation oracle that just counts the number of queries to the oracles -/
 def counting_oracle : simulation_oracle spec spec :=
-{ S := ℕ,
-  o := λ i ⟨t, n⟩, do { u ← query i t, return ⟨u, n + 1⟩ },
-  default_state := 0 }
+⟪ query | λ n _ _ _, n + 1 , 0 ⟫
+
+namespace counting_oracle
+
+section support
+
+end support
+
+section distribution_semantics
+
+section equiv
+
+end equiv
+
+section prob_event
+
+
+end prob_event
+
+end distribution_semantics
+
+end counting_oracle
