src/computational_monads/simulation_semantics/constructions/identity_oracle.lean
@@ -1,8 +1,19 @@
 import computational_monads.simulation_semantics.constructions.stateless_oracle
 
+/-!
+# Identity Oracle
+
+Defines a `simulation_oracle` that just acts as an identity,
+  e.g. simulation with this oracle has no effect (besides an empty state)
+
+Main use cases is in simulating a pair of oracles, where only one of the oracles is reduced.
+  For example preserving a `uniform_selecting` oracle while reducing a `signing_oracle`
+-/
+
 open oracle_comp oracle_spec
 
-variables {A B : Type} {spec spec' spec'' : oracle_spec}
+variables {α β : Type} {spec spec' spec'' : oracle_spec}
+  (oa : oracle_comp spec α) (ob : α → oracle_comp spec β) (s : unit)
 
 @[simps]
 def identity_oracle (spec : oracle_spec) : simulation_oracle spec spec :=
@@ -12,22 +23,17 @@ notation `idₛ` := identity_oracle _
 
 namespace identity_oracle
 
-section instances
-
-instance S_unique : unique (identity_oracle spec).S :=
-punit.unique
-
-end instances
+instance S_unique : unique (identity_oracle spec).S := punit.unique
 
 @[simp]
 lemma apply (i : spec.ι) (t : spec.domain i) (s : unit) :
-  (identity_oracle spec).o i (t, s) = query i t >>= λ u, return (u, ()) := rfl
+  (idₛ).o i (t, s) = query i t >>= λ u, return (u, ()) := rfl
 
 section support
 
 @[simp]
-lemma support_apply (i : spec.ι) (t : spec.domain i) (s : unit) :
-  ((identity_oracle spec).o i (t, s)).support = { u | u.1 ∈ (query i t).support } :=
+lemma support_apply (i : spec.ι) (t : spec.domain i) :
+  ((idₛ).o i (t, s)).support = { u | u.1 ∈ (query i t).support } :=
 begin
   simp only [apply, support_bind, support_pure, set.Union_true,
     set.Union_singleton_eq_range, support_query, set.top_eq_univ, set.mem_univ, set.set_of_true],
@@ -36,26 +42,24 @@ begin
 end
 
 @[simp]
-theorem support_simulate (oa : oracle_comp spec A) (s : unit) :
-  (simulate idₛ oa s).support = {x | x.1 ∈ oa.support} :=
+theorem support_simulate : (simulate idₛ oa s).support = {x | x.1 ∈ oa.support} :=
 begin
   induction oa with A a A B oa ob hoa hob i t generalizing s,
   { ext x,
     simp [prod.eq_iff_fst_eq_snd_eq, punit_eq x.snd (), punit_eq () s] },
   { ext x,    
-    simp only [hoa, hob, unique.exists_iff, bind'_eq_bind, simulate_bind, support_bind, set.mem_set_of_eq, set.mem_Union,
-      prod.exists] },
+    simp only [hoa, hob, unique.exists_iff, bind'_eq_bind, simulate_bind, support_bind,
+      set.mem_set_of_eq, set.mem_Union, prod.exists] },
   { rw [simulate_query, support_apply] }
 end
 
 @[simp]
-lemma mem_support_simulate_iff (oa : oracle_comp spec A) (s : unit) (x : A × unit) :
+lemma mem_support_simulate_iff (x : α × unit) :
   x ∈ (simulate idₛ oa s).support ↔ x.1 ∈ oa.support :=
 by simpa
 
 @[simp]
-lemma support_simulate' (oa : oracle_comp spec A) (s : unit) :
-  (simulate' idₛ oa s).support = oa.support :=
+lemma support_simulate' : (simulate' idₛ oa s).support = oa.support :=
 begin
   ext x,
   simp only [support_simulate', support_simulate, set.mem_image, set.mem_set_of_eq,
@@ -64,43 +68,41 @@ end
 
 end support
 
-section equiv
+section distribution_semantics
 
 open distribution_semantics
 
 variable [spec.finite_range]
 
+section equiv
+
 @[simp]
-lemma apply_equiv (i : spec.ι) (t : spec.domain i) (s : unit) :
-  (identity_oracle spec).o i (t, s) ≃ₚ (λ u, (u, ())) <$> query i t :=
+lemma apply_equiv (i : spec.ι) (t : spec.domain i) :
+  (idₛ).o i (t, s) ≃ₚ (λ u, (u, ())) <$> query i t :=
 rfl
 
 @[simp]
-theorem simulate_equiv (oa : oracle_comp spec A) (s : unit) :
-  simulate idₛ oa s ≃ₚ (λ a, (a, ())) <$> oa :=
+theorem simulate_equiv : simulate idₛ oa s ≃ₚ (λ a, (a, ())) <$> oa :=
 begin
   induction oa with A a A B oa ob hoa hob i t generalizing s,
   { simp [punit_eq s ()] },
   { exact trans (simulate_bind_equiv idₛ oa ob s) (trans (bind_equiv_of_equiv_of_equiv
       (hoa s) (λ x, hob x.fst x.snd)) (by simp)) },
-  { exact (simulate_query_equiv idₛ i t ()).trans (apply_equiv i t ()) }
+  { exact (simulate_query_equiv idₛ i t ()).trans (apply_equiv () i t) }
 end
 
-lemma default_simulate_equiv (oa : oracle_comp spec A) (s : unit) :
-  default_simulate idₛ oa ≃ₚ (λ a, (a, ())) <$> oa :=
+lemma default_simulate_equiv : default_simulate idₛ oa ≃ₚ (λ a, (a, ())) <$> oa :=
 simulate_equiv oa ()
 
 @[simp]
-lemma simulate'_identity_oracle_equiv (oa : oracle_comp spec A) (s : unit) :
-  (simulate' idₛ oa s) ≃ₚ oa :=
+lemma simulate'_equiv : (simulate' idₛ oa s) ≃ₚ oa :=
 calc simulate' idₛ oa s ≃ₚ prod.fst <$> simulate idₛ oa s : rfl
   ... ≃ₚ prod.fst <$> (λ a, (a, ())) <$> oa : (map_equiv_of_equiv _ (simulate_equiv oa s))
   ... ≃ₚ (prod.fst ∘ λ a, (a, ())) <$> oa : map_map_equiv oa _ _
   ... ≃ₚ oa : map_equiv_of_eq_id _ _ (by simp)
 
-lemma default_simulate'_equiv (oa : oracle_comp spec A) (s : unit) :
-  default_simulate' idₛ oa ≃ₚ oa :=
-simulate'_identity_oracle_equiv oa ()
+lemma default_simulate'_equiv : default_simulate' idₛ oa ≃ₚ oa :=
+simulate'_equiv oa ()
 
 end equiv
 
@@ -110,6 +112,6 @@ section prob_event
 
 end prob_event
 
-
+end distribution_semantics
 
 end identity_oracle
